Garden/OpenVM/Sha256/air_expr.v
@@ -110,7 +110,7 @@ Definition eval_row (start_col : Z) (local_cols : Sha256DigestCols.t Var.t) : ME
 Definition print_eval_row : string :=
   let start_col := 0 in
   let local_cols : Sha256DigestCols.t Var.t :=
-    MGenerateVar.eval MGenerateVar.generate in
+    MGenerate.eval MGenerate.generate in
   ToRocq.cats [
     ToRocq.endl;
     ToRocq.to_rocq (eval_row start_col local_cols) 0;
@@ -817,19 +817,19 @@ Definition print_eval : string :=
   |} in
   let start_col := 0 in
   let '(round_local_cols, round_next_cols) :=
-    MGenerateVar.eval [[ (
-      MGenerateVar.generate (A := Sha256RoundCols.t Var.t) (||),
-      MGenerateVar.generate (A := Sha256RoundCols.t Var.t) (||)
+    MGenerate.eval [[ (
+      MGenerate.generate (A := Sha256RoundCols.t Var.t) (||),
+      MGenerate.generate (A := Sha256RoundCols.t Var.t) (||)
     ) ]] in
   (* Because the "round" version is longer than the "digest" one *)
   let digest_local_cols :=
-    MGenerateVar.eval [[
-      MGenerateVar.generate (A := Sha256DigestCols.t Var.t) (||)
+    MGenerate.eval [[
+      MGenerate.generate (A := Sha256DigestCols.t Var.t) (||)
     ]] in
   let '(_, digest_next_cols) :=
-    MGenerateVar.eval [[ (
-      MGenerateVar.generate (A := Sha256RoundCols.t Var.t) (||),
-      MGenerateVar.generate (A := Sha256DigestCols.t Var.t) (||)
+    MGenerate.eval [[ (
+      MGenerate.generate (A := Sha256RoundCols.t Var.t) (||),
+      MGenerate.generate (A := Sha256DigestCols.t Var.t) (||)
     ) ]] in
   ToRocq.cats [
     ToRocq.endl;
